Rga as n-ary tree - wip

inductive_proof/Rga/App_do_pre_merge_pre.fst
@@ -4,27 +4,255 @@ open SeqUtils
 module L = FStar.List.Tot
 
 type node =
-| Leaf 
+//| Leaf 
 | Node : (pos & nat) -> list node -> node
 
-type concrete_st =
-| Root : list node -> concrete_st
+type concrete_st' =
+| Root : list node -> concrete_st'
 
-let (a:concrete_st) = (Root [(Node (1,0) [Leaf])])
-
-let get_lst (s:concrete_st) = 
+let get_lst (s:concrete_st') = 
   let Root l = s in l
 
-let rec mem' (value:(pos * nat)) (l:list node) =
+let rec mem' (value:(pos & nat)) (l:list node) =
   match l with
   |[] -> false
   |x::xs -> match x with
-          |Leaf -> false
+          //|Leaf -> false
           |Node x lst -> value = x || mem' value lst || mem' value xs
 
-let mem (value:(pos * nat)) (s:concrete_st) = mem' value (get_lst s)
+let mem (value:(pos & nat)) (s:concrete_st') = mem' value (get_lst s)
+
+let rec mem_id_s' (id:pos) (l:list node) 
+  : Tot (b:bool{b = true <==> (exists ele. mem' (id, ele) l)}) =
+  match l with
+  |[] -> false
+  |x::xs -> match x with
+          //|Leaf -> false
+          |Node (v,_) lst -> id = v || mem_id_s' id lst || mem_id_s' id xs
+
+let mem_id_s (id:pos) (s:concrete_st') = mem_id_s' id (get_lst s)
+
+let _ = assert (mem_id_s 1 (Root 
+                            [(Node (4,1) 
+                              [(Node (1,1) [])]); 
+                               (Node (1,1) []); 
+                                ]))
+
+let rec unique_st' (l:list node) =
+  match l with
+  |[] -> True
+  |x::xs -> match x with
+          //|Leaf -> True
+          |Node (id,_) lst -> not (mem_id_s' id lst) /\ not (mem_id_s' id xs) /\ unique_st' lst /\ unique_st' xs
+                             /\ (forall id. mem_id_s' id xs ==> not (mem_id_s' id lst))
+
+let rec count (id:pos) (l:list node) : nat =
+  match l with
+  | [] -> 0
+  | x::xs -> match x with
+           //|Leaf -> count id xs
+           |Node (node_id, _) xs' -> let rest_count = count id xs in
+                                    let rest_count' = count id xs' in
+                                    let node_count = if node_id = id then 1 else 0 in
+                                    rest_count + node_count + rest_count'
+
+let _ = assert (count 1 [(Node (2,1) 
+                           [(Node (1,1) [])]);
+                         (Node (1,1) []); 
+                         (Node (1,1) [])] = 3)
+
+let unique_st (s:concrete_st') = unique_st' (get_lst s)
+
+type concrete_st = s:concrete_st'{unique_st s}
 
 let _ = assert (mem (4,1) (Root [(Node (4,1) [(Node (2,1) [])]); (Node (3,1) [])]))
+
+// init state
+let init_st = (Root [])
+
+// equivalence between 2 concrete states
+let eq (a b:concrete_st) = a == b
+
+// few properties of equivalence relation
+let symmetric (a b:concrete_st) 
+  : Lemma (requires eq a b)
+          (ensures eq b a) = ()
+
+let transitive (a b c:concrete_st)
+  : Lemma (requires eq a b /\ eq b c)
+          (ensures eq a c) = ()
+
+let eq_is_equiv (a b:concrete_st)
+  : Lemma (requires a == b)
+          (ensures eq a b) = ()
+
+// operation type
+// (the only operation is Add, so nat is fine)
+type app_op_t:eqtype = 
+  |Add_after : after_id:nat -> ele:nat -> app_op_t //inserts ele after after_id
+
+let get_after_id (o:op_t) : nat =
+  let (_, Add_after id _) = o in id
+
+let get_ele (o:op_t) : nat =
+  let (_, Add_after _ ele) = o in ele
+  
+let do_pre (s:concrete_st) (o:op_t) =
+  let (ts, Add_after after_id _) = o in
+  ~ (mem_id_s ts s) /\
+  (~ (after_id = 0) ==> mem_id_s after_id s)
+
+let rec contains_child (child:(pos & nat)) (children:list node) =
+  match children with
+  |[] -> false
+  |x::xs -> match x with
+          //|Leaf -> contains_child child xs
+          |Node y _ -> child = y || contains_child child xs
+
+//immediate child
+let rec is_child (child:(pos & nat)) (parent:pos) (l:list node) =
+  match l with
+  |[] -> false
+  |x::xs -> match x with
+          //|Leaf -> is_child child parent xs
+          |Node x children -> if fst x = parent then contains_child child children 
+                             else (is_child child parent children || is_child child parent xs)
+
+let rec get_children (id:pos) (l:list node{mem_id_s' id l /\ unique_st' l}) = 
+  match l with
+  |x::xs -> match x with
+          |Node value children -> if fst value = id then children 
+                                 else if mem_id_s' id children then get_children id children
+                                 else get_children id xs
+
+let rec get_chldn_lst (l:list node) =
+  match l with
+  |[] -> []
+  |(Node v _)::xs -> v::get_chldn_lst xs
+
+let rec get_children_lst (id:pos) (l:list node{mem_id_s' id l /\ unique_st' l}) =
+  match l with
+  |Node value chldn::xs -> if fst value = id then get_chldn_lst chldn 
+                         else if mem_id_s' id chldn then get_children_lst id chldn
+                         else get_children_lst id xs
+
+let rec lem_same (l l1:list node) 
+  : Lemma (requires unique_st' l /\ unique_st' l1 /\
+                    (get_chldn_lst l = get_chldn_lst l1) /\
+                    (forall id. mem_id_s' id l /\ mem_id_s' id l1 ==>
+                           get_children_lst id l = get_children_lst id l1))
+          (ensures l = l1) 
+          (decreases %[l;l1]) =
+  match l, l1 with
+  |[],[] -> ()
+  |[],_ |_,[] -> ()
+  |Node p1 c1::xs, Node p2 c2::ys -> lem_same c1 c2; lem_same xs ys
+  
+let check' (l:list node)
+  : Lemma (requires l == [(Node (2,1) 
+                           [(Node (4,1) 
+                             [(Node (5,1) 
+                               [(Node (6,1) []);
+                                (Node (7,1) [])])]);
+                            (Node (10,1) [])]);
+                         (Node (1,1) []); 
+                         (Node (3,1) [])])
+          (ensures mem_id_s' 3 l /\ unique_st' l /\ get_children 5 l = [(Node (6,1) []);
+                                                                      (Node (7,1) [])]) = ()
+          
+let rec is_sibling (s1 s2:(pos * nat)) (l:list node) =
+  match l with
+  |[] -> false 
+  |[x] -> (match x with
+         //|Leaf -> false
+         |Node y children -> is_sibling s1 s2 children)
+  |x::y::xs -> match x,y with
+            //|Leaf, Leaf -> is_sibling s1 s2 xs
+            //|Leaf, _ -> is_sibling s1 s2 (y::xs)
+            //|_, Leaf -> is_sibling s1 s2 xs
+            |Node x1 chld1, Node x2 chld2 -> (x1 = s1 && x2 = s2) || is_sibling s1 s2 chld1
+                                            || is_sibling s1 s2 chld2 || is_sibling s1 s2 (y::xs)
+
+let check (l:list node)
+  : Lemma (requires l == [(Node (2,1) 
+                           [(Node (4,1) 
+                             [(Node (5,1) 
+                               [(Node (6,1) [])])])]);
+                         (Node (1,1) []); 
+                         (Node (3,1) [])])
+          (ensures is_child (6,1) 5 l /\ not (is_child (5,1) 2 l)) = ()
+
+let check1 (l:list node)
+  : Lemma (requires l == [(Node (2,1) 
+                           [(Node (4,1) 
+                             [(Node (5,1) 
+                               [(Node (6,1) []);
+                                (Node (7,1) [])])]);
+                            (Node (10,1) [])]);
+                         (Node (1,1) []); 
+                         (Node (3,1) [])])
+          (ensures is_sibling (4,1) (10,1) l) = ()
+          
+#push-options "--z3rlimit 50 --ifuel 1"
+let rec add_after_id (l:list node{unique_st' l}) 
+                     (ts:pos{not (mem_id_s' ts l)}) 
+                     (after_id:pos{mem_id_s' after_id l}) 
+                     (ele:nat) 
+   : Tot (r:list node{unique_st' r /\ mem_id_s' ts r /\
+                      (forall id. mem_id_s' id r <==> mem_id_s' id l \/ id = ts) /\
+                      is_child (ts, ele) after_id r /\
+                      get_children_lst after_id r = (ts, ele)::get_children_lst after_id l /\
+                      get_chldn_lst l = get_chldn_lst r /\
+                      (forall id. mem_id_s' id l /\ id <> after_id ==>
+                         (get_children_lst id l = get_children_lst id r))})
+     (decreases l) =
+  match l with
+  |x::xs -> if mem_id_s' after_id [x] then 
+    (let child' = (match x with
+                  |Node value children -> if fst value = after_id 
+                                        then (assert (forall id. mem_id_s' id children ==>
+                                                            get_children_lst id l = get_children_lst id children);
+                                              Node value (Node (ts,ele) []::children))
+                                        else (assert (mem_id_s' after_id children); 
+                                              Node value (add_after_id children ts after_id ele))) in
+                                        
+      (assert (not (mem_id_s' after_id xs)); 
+       assert (forall id. mem_id_s' id xs ==> get_children_lst id xs = get_children_lst id l);
+       let r = child'::xs in
+       assert (is_child (ts,ele) after_id r);
+       assert (mem_id_s' ts r); 
+       assert (unique_st' r);
+       assert (forall id. mem_id_s' id l /\ id <> after_id ==>
+                         (get_children_lst id l = get_children_lst id r)); 
+       r))
+    else
+    (let r = x::(add_after_id xs ts after_id ele) in 
+     assert (is_child (ts,ele) after_id r);
+     assert (mem_id_s' ts r); 
+     assert (unique_st' r);
+     r)
+
+let do (s:concrete_st) (op:op_t{do_pre s op}) 
+  : (r:concrete_st{(get_after_id op = 0 ==> 
+         get_chldn_lst (get_lst r) = (fst op, get_ele op)::get_chldn_lst (get_lst s) /\
+         (forall id. mem_id_s' id (get_lst s) /\ mem_id_s' id (get_lst r) ==>
+                get_children_lst id (get_lst s) = get_children_lst id (get_lst r)))}) =
+  
+  let (ts, Add_after after_id ele) = op in
+  if after_id = 0 then (Root ((Node (ts, ele) [])::(get_lst s)))
+  else (Root (add_after_id (get_lst s) ts after_id ele))
+
+let lem_do (a b:concrete_st) (op:op_t)
+   : Lemma (requires eq a b /\ do_pre a op)
+           (ensures eq (do a op) (do b op)) = ()
+
+//conflict resolution
+let resolve_conflict (x:op_t) (y:op_t{fst x <> fst y}) : resolve_conflict_res = 
+  match x, y with
+  |(ts1, (Add_after id1 _)), (ts2, (Add_after id2 _)) -> if id1 = id2 then 
+                                                           if ts1 > ts2 then First_then_second else Second_then_first 
+                                                        else First_then_second //ts1 <> id2 /\ ts2 <> id1
+
 
 (*
 type concrete_st' = 
